src/Assembly/Equivalence.v
@@ -413,17 +413,16 @@ Proof.
             let lu := Z.log2 u in
             if (Z.eqb l 0 && Z.eqb u (2^lu))%bool
             then
-              (* App (((slice 0 (Z.to_N lu)), Z.to_N lu, [idx])) *)
-              symex_return idx
+              App (((slice 0 (Z.to_N lu)), Some (Z.to_N lu), [idx])) 
             else symex_error (Unhandled_cast l u)
           in
           match idc in ident t return symex_T t with
           | ident.Literal base.type.Z v
-            => App (const (Z.to_N v), Some 64%N, nil) (* note: 64 is placeholder, to_N is unsound *)
-          | ident.Z_add => fun x y => App (add, Some 64%N, [x; y])
+            => App (const (Z.to_N v), None, nil) (* note: 64 is placeholder, to_N is unsound *)
+          | ident.Z_add => fun x y => App (add, None, [x; y])
 
           | ident.Z_modulo
-          | ident.Z_mul => fun x y => App (mul, Some 64%N, [x; y])
+          | ident.Z_mul => fun x y => App (mul, None, [x; y])
           | ident.Z_pow
           | ident.Z_sub
           | ident.Z_opp
@@ -432,28 +431,28 @@ Proof.
           | ident.Z_log2_up
           | ident.Z_to_nat
             => symex_T_error (Unhandled_identifier idc)
-          | ident.Z_shiftr => fun x y => App (shr, Some 64%N, [x; y])
-          | ident.Z_shiftl => fun x y => App (shl, Some 64%N, [x; y])
-          | ident.Z_land => fun x y => App (and, Some 64%N, [x; y])
-          | ident.Z_lor => fun x y => App (or, Some 64%N, [x; y])
+          | ident.Z_shiftr => fun x y => App (shr, None, [x; y])
+          | ident.Z_shiftl => fun x y => App (shl, None, [x; y])
+          | ident.Z_land => fun x y => App (and, None, [x; y])
+          | ident.Z_lor => fun x y => App (or, None, [x; y])
           | ident.Z_min
           | ident.Z_max
             => symex_T_error (Unhandled_identifier idc)
            (* note for mulhuu/adc: the argument and output order is a guess, 64 is a kludge and we need something better to use the value of s whose type is var *)
           | ident.Z_mul_split => fun s x y =>
-            lo <- App (mul, Some 64%N, [x; y]);
-            hi <- App (mulhuu 64%N, Some 64%N, [x; y]);
+            lo <- App (mul, None, [x; y]);
+            hi <- App (mulhuu 64%N, None, [x; y]);
             symex_return (lo, hi)
-          | ident.Z_mul_high => fun s x y => App (mulhuu 64%N, Some 64%N, [x; y])
+          | ident.Z_mul_high => fun s x y => App (mulhuu 64%N, None, [x; y])
           | ident.Z_add_get_carry => fun s x y =>
-            a <- App (add     , Some 64%N, [x; y]);
-            c <- App (addcarry, Some 64%N, [x; y]);
+            a <- App (add     , None, [x; y]);
+            c <- App (addcarry, None, [x; y]);
             symex_return (a, c)
-          | ident.Z_add_with_carry => fun x y z => App (add, Some 64%N, [x; y; z])
+          | ident.Z_add_with_carry => fun x y z => App (add, None, [x; y; z])
 
           | ident.Z_add_with_get_carry => fun s x y z =>
-            a <- App (add     , Some 64%N, [x; y; z]);
-            c <- App (addcarry, Some 64%N, [x; y; z]);
+            a <- App (add     , None, [x; y; z]);
+            c <- App (addcarry, None, [x; y; z]);
             symex_return (a, c)
           | ident.Z_sub_get_borrow
           | ident.Z_sub_with_get_borrow
@@ -462,7 +461,7 @@ Proof.
           | ident.Z_add_modulo
             => symex_T_error (Unhandled_identifier idc)
             (* assuming s=64 *)
-          | ident.Z_truncating_shiftl => fun s x y => App (shl, Some 64%N, [x; y])
+          | ident.Z_truncating_shiftl => fun s x y => App (shl, None, [x; y])
           | ident.Z_bneg
           | ident.Z_lnot_modulo
           | ident.Z_lxor
@@ -533,7 +532,7 @@ Proof.
                   idx2 <- symex_mod_zrange v2_idx r2;
                   symex_return (idx1, idx2)
           | ident.Z_of_nat
-            => fun n => App (const (N.of_nat n), Some 64%N, nil) (* note: 64 is placeholder *)
+            => fun n => App (const (N.of_nat n), None, nil) (* note: 64 is placeholder *)
 
           | ident.Z_eqb
           | ident.Z_leb
